Begin entering the code for System F

src/Sem.v
@@ -14,23 +14,17 @@ From Equations Require Import Equations.
 Require Import Equations.Type.EqDec.
 Set Equations With UIP.
 
+Require Import Lam.
+
 Generalizable All Variables.
 
 Import ListNotations.
-
-Inductive Ty :=
-  | TUnit
-  | TFunc : Ty → Ty → Ty.
-
-Infix "⟶" := TFunc (at level 30, right associativity).
 
 Fixpoint SemTy (τ : Ty) : Type :=
   match τ with
   | TUnit => unit
   | TFunc dom cod => SemTy dom → SemTy cod
   end.
-
-Definition Env := list Ty.
 
 Fixpoint SemEnv E : Type :=
   match E with
@@ -47,134 +41,9 @@ Fixpoint SemEnv E : Type :=
 (* Notation "·" := Empty. *)
 (* Notation "Γ ⸴ A ： τ" := (@Cons τ A _ _ Γ) (at level 80, right associativity). *)
 
-Inductive Var : Env → Ty → Set :=
-  | ZV Γ τ    : Var (τ :: Γ) τ
-  | SV Γ τ τ' : Var Γ τ → Var (τ' :: Γ) τ.
-
-Arguments ZV {_ _}.
-Arguments SV {_ _ _} _.
-
-(* Notation "Γ ∋ A ： τ" := (@Var _ _ Γ τ A) (at level 80, no associativity). *)
-
-Inductive Exp Γ : Ty → Set :=
-  | VAR {τ}       : Var Γ τ → Exp Γ τ
-  | ABS {dom cod} : Exp (dom :: Γ) cod → Exp Γ (dom ⟶ cod)
-  | APP {dom cod} : Exp Γ (dom ⟶ cod) → Exp Γ dom → Exp Γ cod.
-
-Arguments VAR {Γ τ} _.
-Arguments ABS {Γ dom cod} _.
-Arguments APP {Γ dom cod} _ _.
-
-Definition Sub Γ Γ' := ∀ {τ}, Var Γ τ → Exp Γ' τ.
-
-Definition idSub {Γ} : Sub Γ Γ := @VAR Γ.
-
-(*
-Program Definition consSub {Γ Γ' τ} (e : Exp Γ' τ)
-        (s : Sub Γ Γ') : Sub (τ :: Γ) Γ' :=
-  λ _ v, match v with
-         | ZV    => e
-         | SV v' => s _ v'
-         end.
-*)
-
-Equations consSub {Γ Γ' τ} (e : Exp Γ' τ) (s : Sub Γ Γ')
-          τ' (v : Var (τ :: Γ) τ') : Exp Γ' τ' :=
-  consSub e s τ' ZV      := e;
-  consSub e s τ' (SV v') := s _ v'.
-
-Notation "{| e ; .. ; f |}" := (consSub e .. (consSub f idSub) ..).
-
-Definition tlSub {Γ Γ' τ} (s : Sub (τ :: Γ) Γ') : Sub Γ Γ' :=
-  fun τ' v => s τ' (SV v).
-Definition hdSub {Γ Γ' τ} (s : Sub (τ :: Γ) Γ') : Exp Γ' τ := s τ ZV.
-
-Definition Ren Γ Γ' := ∀ {τ}, Var Γ τ → Var Γ' τ.
-
-Definition idRen {Γ} : Ren Γ Γ := λ _, id.
-
-Definition tlRen {Γ Γ' τ} (r : Ren (τ :: Γ) Γ') : Ren Γ Γ' :=
-  fun τ' v => r τ' (SV v).
-Definition hdRen {Γ Γ' τ} (r : Ren (τ :: Γ) Γ') : Var Γ' τ := r τ ZV.
-
-Definition skip1 {Γ τ} : Ren Γ (τ :: Γ) := λ _, SV.
-
-Equations skipn {Γ} Γ' : Ren Γ (Γ' ++ Γ) :=
-  skipn []        := λ _, id;
-  skipn (x :: xs) := λ τ v, SV (skipn xs τ v).
-
 Equations trunc {Γ} Γ' `(E : SemEnv (Γ' ++ Γ)) : SemEnv Γ :=
   trunc []        E := E;
   trunc (x :: xs) E := trunc xs (snd E).
-
-(*
-Program Definition RTmL {Γ Γ' τ} (r : Ren Γ Γ') :
-        Ren (τ :: Γ) (τ :: Γ') :=
-  λ _ v, match v with
-         | ZV    => ZV
-         | SV v' => SV (r _ v')
-         end.
-*)
-
-(* This version gives better rewriting equations. *)
-Equations RTmL {Γ Γ' τ} (r : Ren Γ Γ')
-          τ' (v : Var (τ :: Γ) τ') : Var (τ :: Γ') τ' :=
-  RTmL r τ' ZV      := ZV;
-  RTmL r τ' (SV v') := SV (r _ v').
-
-Lemma RTmL_id {Γ τ} : @RTmL Γ Γ τ (λ _, id) = λ _, id.
-Proof.
-  extensionality τ'.
-  extensionality v.
-  dependent induction v.
-  - now rewrite RTmL_equation_1.
-  - now rewrite RTmL_equation_2.
-Qed.
-
-Fixpoint RTmExp {Γ Γ' τ} (r : Ren Γ Γ') (e : Exp Γ τ) : Exp Γ' τ :=
-  match e with
-  | VAR v     => VAR (r _ v)
-  | APP e1 e2 => APP (RTmExp r e1) (RTmExp r e2)
-  | ABS e     => ABS (RTmExp (RTmL r) e)
-  end.
-
-Definition wk {Γ τ τ'} : Exp Γ τ → Exp (τ' :: Γ) τ := RTmExp (λ _, SV).
-
-(*
-Program Definition STmL {Γ Γ' τ} (s : Sub Γ Γ') :
-        Sub (τ :: Γ) (τ :: Γ') :=
-  λ _ v, match v with
-         | ZV    => VAR ZV
-         | SV v' => wk (s _ v')
-         end.
-*)
-
-Equations STmL {Γ Γ' τ} (s : Sub Γ Γ') τ' (v : Var (τ :: Γ) τ') :
-  Exp (τ :: Γ') τ' :=
-  STmL _ τ' ZV      := VAR ZV;
-  STmL _ τ' (SV v') := wk (s _ v').
-
-Fixpoint STmExp {Γ Γ' τ} (s : Sub Γ Γ') (e : Exp Γ τ) : Exp Γ' τ :=
-  match e with
-  | VAR v     => s _ v
-  | APP e1 e2 => APP (STmExp s e1) (STmExp s e2)
-  | ABS e     => ABS (STmExp (STmL s) e)
-  end.
-
-Inductive Ev : ∀ {τ}, Exp [] τ → Exp [] τ → Prop :=
-  | EvAbs t1 t2 (e : Exp [t1] t2) : Ev (ABS e) (ABS e)
-  | EvApp t1 t2 e v w (e1 : Exp [] (t1 ⟶ t2)) e2 :
-    Ev e1 (ABS e) → Ev e2 w → Ev (STmExp {| w |} e) v →
-    Ev (APP e1 e2) v.
-
-(* Notation "Γ ⊢ e ： τ" := (Judgment Γ τ e) (at level 80, no associativity). *)
-
-Definition identity Γ τ : Exp Γ (τ ⟶ τ) := ABS (VAR ZV).
-
-Definition compose {Γ τ τ' τ''}
-           (f : Exp Γ (τ' ⟶ τ''))
-           (g : Exp Γ (τ ⟶ τ')) : Exp Γ (τ ⟶ τ'') :=
-  ABS (APP (wk f) (APP (wk g) (VAR ZV))).
 
 Fixpoint SemVar `(v : Var Γ τ) : SemEnv Γ → SemTy τ :=
   match v with
@@ -225,26 +94,6 @@ Proof.
   - now rewrite IHe1, IHe2.
 Qed.
 
-Definition RcR {Γ Γ' Γ''} (r : Ren Γ' Γ'') (r' : Ren Γ Γ') :=
-  (λ τ v, r τ (r' τ v)) : Ren Γ Γ''.
-
-Definition ScR {Γ Γ' Γ''} (s : Sub Γ' Γ'') (r : Ren Γ Γ') :=
-  (λ τ v, s τ (r τ v)) : Sub Γ Γ''.
-
-Definition RcS {Γ Γ' Γ''} (r : Ren Γ' Γ'') (s : Sub Γ Γ') :=
-  (λ τ v, RTmExp r (s τ v)) : Sub Γ Γ''.
-
-Definition ScS {Γ Γ' Γ''} (s : Sub Γ' Γ'') (s' : Sub Γ Γ') :=
-  (λ τ v, STmExp s (s' τ v)) : Sub Γ Γ''.
-
-Lemma LiftRcR Γ Γ' Γ'' τ (r : Ren Γ' Γ'') (r' : Ren Γ Γ') :
-  RTmL (τ := τ) (RcR r r') = RcR (RTmL r) (RTmL r').
-Proof.
-  extensionality τ'.
-  extensionality v.
-  now dependent induction v.
-Qed.
-
 Lemma SemRenVarComm Γ τ (v : Var Γ τ) Γ' (r : Ren Γ Γ') :
   ∀ se, SemVar v (SemRen r se) = SemVar (r _ v) se.
 Proof.
@@ -285,10 +134,6 @@ Proof.
     unfold skip1, RcR in IHΓ''.
     now rewrite <- IHΓ''.
 Qed.
-
-Corollary tlRen_skip1 Γ τ τ' :
-  @tlRen _ (τ :: τ' :: Γ) _ skip1 = RcR skip1 skip1.
-Proof. reflexivity. Qed.
 
 Lemma SemRen_skip1 (Γ : Env) (τ : Ty) :
   SemRen skip1 = @snd (SemTy τ) (SemEnv Γ).
