src/Db.v
@@ -1,0 +1,126 @@
+Require Import
+  Coq.Program.Program
+  Coq.Unicode.Utf8
+  Coq.micromega.Lia
+  Coq.Classes.Morphisms
+  Coq.Relations.Relation_Definitions
+  Coq.Strings.String
+  Coq.Vectors.Vector
+  Coq.Lists.List
+  Coq.Sets.Ensembles
+  Coq.Logic.EqdepFacts.
+
+From Equations Require Import Equations.
+Require Import Equations.Type.EqDec.
+Set Equations With UIP.
+
+Set Universe Polymorphism.
+
+Generalizable All Variables.
+
+Import ListNotations.
+
+Definition stream (A : Type) : Type := nat → A.
+
+Definition result_stream `(S : stream A) (B : A → Type) : Type :=
+  ∀ n : nat, B (S n).
+
+Definition dep_stream (A : Type) (B : A → Type) : Type :=
+  ∀ S : stream A, result_stream S B.
+
+Definition Schema : Type := list (string * Type).
+
+Inductive Rec : Schema → Type :=
+  | Empty : Rec []
+  | Field name {ty S} : ty → Rec S → Rec ((name, ty) :: S).
+
+(* jww (2022-06-15): Keys are just unique names at the moment *)
+Definition Table (S : Schema) : Type := list (string * Rec S).
+
+Open Scope string_scope.
+
+Example same_record :
+  Rec [("foo", nat : Type); ("bar", nat : Type); ("baz", nat : Type)].
+Proof.
+  exact (Field "foo" (1 : nat)
+               (Field "bar" (2 : nat)
+                      (Field "baz" (3 : nat) Empty))).
+Qed.
+
+Definition Database : Type := list (string * { S : Schema & Table S }).
+
+Section Kadena.
+
+Class EqDec (A : Type) := {
+    eq_dec : ∀ x y : A, {x = y} + {x ≠ y}
+}.
+
+Fixpoint lookup {k v : Type} `{EqDec k} (i : k) (l : list (k * v)) : option v :=
+  match l with
+  | [] => None
+  | (j, x) :: xs => if eq_dec i j then Some x else lookup i xs
+  end.
+
+(* At the moment all database operations are "global" and not constrained to
+   what the capabilities of the contract permit it to see. *)
+Inductive Op : Type :=
+  | Noop
+  | Query {a : Type} (q : Database → a)
+  | Update (u : Database → Database).
+
+Inductive Result : Op → Type :=
+  | Nothing : Result Noop
+  | Answer {a} {q : Database → a} : a → Result (Query q)
+  | Updated {u} : Result (Update u)
+  (* Any operation might result in an error. *)
+  | Error {o} (msg : string) : Result o.
+
+Definition Kadena := dep_stream Op Result.
+
+Definition Contract : Type := list Op * Op.
+
+Definition Modules : Schema := [ ("contract", Contract) ].
+
+Definition NoopContract : Contract := ([], Noop).
+Definition NoopModule : Rec Modules := Field "contract" NoopContract Empty.
+
+Program Definition Store : Database :=
+  [ ("modules", existT _ Modules [("noop", NoopModule)]) ].
+
+Definition kda : Kadena.
+Proof.
+  repeat intro.
+  induction (S n); constructor.
+  apply q.
+  exact Store.
+Defined.
+
+Fixpoint typeof {S : Schema} (r : Rec S) (field : string) : Type :=
+  match r with
+  | Empty => False
+  | @Field name ty _ _ xs =>
+      if name =? field then ty else typeof xs field
+  end.
+
+Equations get {S : Schema} (r : Rec S) (field : string) : typeof r field :=
+  get Empty _ := False_rect _ _;
+  get (Field name x xs) field := if name =? field then x else get xs field.
+
+Program Definition call_noop_contract (k : Kadena) :=
+  k (λ n, if Nat.eqb n 0
+          then Update (λ _, Store) (* genesis *)
+          else Query (λ db, match lookup "modules" db with
+                            | Some (existT _ _ ms) =>
+                                match lookup "noop" ms with
+                                | Some r =>
+                                    get r "contract"
+                                | None => Error "failed"
+                                end
+                            | None => Error "failed"
+                            end)) 1.
+
+Lemma call_noop_contract_correct :
+  call_noop_contract kda = Answer ().
+Proof. reflexivity. Qed.
+
+End Kadena.
