src/SysF.v
@@ -1,0 +1,258 @@
+Require Import
+  Coq.Program.Program
+  Coq.Unicode.Utf8
+  Coq.micromega.Lia
+  Coq.Classes.Morphisms
+  Coq.Relations.Relation_Definitions
+  Coq.Strings.String
+  Coq.Vectors.Vector
+  Coq.Lists.List
+  Coq.Sets.Ensembles
+  Coq.Logic.EqdepFacts.
+
+From Equations Require Import Equations.
+Require Import Equations.Type.EqDec.
+Set Equations With UIP.
+
+Generalizable All Variables.
+
+Import ListNotations.
+
+Inductive TyVar : nat → Type := 
+  | ZTYVAR {u} : TyVar (S u) 
+  | STYVAR {u} : TyVar u → TyVar (S u).
+
+Inductive Ty u :=
+  | TYVAR : TyVar u → Ty u
+  | ARR   : Ty u → Ty u → Ty u
+  | ALL   : Ty (S u) → Ty u.
+
+Arguments TYVAR : default implicits.
+Arguments ARR : default implicits.
+Arguments ALL : default implicits.
+
+Infix "⟶" := ARR (at level 30, right associativity).
+
+Definition RenT u w := TyVar u → TyVar w.
+Definition SubT u w := TyVar u → Ty w.
+
+Program Definition RTyL `(r : RenT u w) : RenT (S u) (S w) :=
+  λ v, match v with 
+       | ZTYVAR      => ZTYVAR
+       | STYVAR var' => STYVAR (r var')
+       end.
+
+Fixpoint RTyT `(r : RenT u w) (t : Ty u) : Ty w :=
+  match t with 
+  | TYVAR v   => TYVAR (r v) 
+  | ARR t1 t2 => ARR (RTyT r t1) (RTyT r t2) 
+  | ALL t     => ALL (RTyT (RTyL r) t)
+  end.
+
+Definition ShTyT {u} : Ty u → Ty (S u) := RTyT (@STYVAR _).
+
+Program Definition STyL `(s : SubT u w) : SubT (S u) (S w) :=
+  λ v, match v with 
+       | ZTYVAR    => TYVAR ZTYVAR
+       | STYVAR v' => ShTyT (s v')
+       end.
+
+Fixpoint STyT `(s : SubT u w) (t : Ty u) : Ty w :=
+  match t with
+  | TYVAR v   => s v
+  | ARR t1 t2 => ARR (STyT s t1) (STyT s t2) 
+  | ALL t     => ALL (STyT (STyL s) t)
+  end.
+
+Definition Env u := list (Ty u).
+
+Fixpoint STyE `(sub : SubT u w) (env : Env u) : Env w :=
+  match env with
+  | []      => []
+  | T :: TS => STyT sub T :: STyE sub TS
+  end.
+
+Inductive Var {u} : Env u → Ty u → Set :=
+  | ZVAR {Γ τ}    : Var (τ :: Γ) τ
+  | SVAR {Γ τ τ'} : Var Γ τ → Var (τ' :: Γ) τ.
+
+Arguments ZVAR : default implicits.
+Arguments SVAR : default implicits.
+
+Definition shSubT {u} : SubT u (S u) := λ v, TYVAR (STYVAR v).
+
+(* Notation "Γ ∋ A ： τ" := (@Var _ _ Γ τ A) (at level 80, no associativity). *)
+
+Definition idSubT {Γ} : SubT Γ Γ := @TYVAR Γ.
+
+Equations consSubT {u w} (e : Ty u) (s : SubT u w)
+          (v : TyVar w) : Ty w :=
+  consSubT e s ZTYVAR      := e;
+  consSubT e s (STYVAR v') := s _ v'.
+
+Notation "{| e ; .. ; f |}" := (consSub e .. (consSub f idSub) ..).
+
+Inductive Exp `(Γ : Env u) : Ty u → Type :=
+  | VAR {τ}       : Var Γ τ → Exp Γ τ
+  | LAM {dom cod} : Exp (dom :: Γ) cod → Exp Γ (dom ⟶ cod)
+  | APP {dom cod} : Exp Γ (dom ⟶ cod) → Exp Γ dom → Exp Γ cod
+  | TAPP {τ}      : Exp Γ (ALL τ) → ∀ τ' : Ty u, Exp Γ (STyT [| τ' |] τ)
+  | TLAM {τ}      : Exp (u:=S u) (STyE (shSubT _) Γ) τ → Exp Γ (ALL τ).
+
+Arguments VAR : default implicits
+Arguments LAM : default implicits
+Arguments APP : default implicits.
+Arguments TAPP : default implicits.
+Arguments TLAM : default implicits.
+
+Lemma STyExp_cast1 `(sub : SubT u w) (env : Env u)
+      (ty : Ty (S u)) (ty' : Ty u) :
+  @eq Type
+      (Exp (STyE sub env) (STyT [| STyT sub ty' |] (STyT (STyL sub) ty)))
+      (Exp (STyE sub env) (STyT sub (STyT [| ty' |] ty))).
+
+Lemma STyExp_cast2 `(sub : SubT u w) (env : Env u) (ty : Ty (S u)),
+  @eq Type
+      (Exp (STyE (STyL sub) (STyE (shSubT u) env)) (STyT (STyL sub) ty))
+      (Exp (STyE (shSubT _) (STyE sub env)) (STyT (STyL sub) ty)).
+
+Fixpoint STyExp u w (s : SubT u w) (E : Env u) t (e : Exp E t) :
+  Exp (STyE s E) (STyT s t) :=
+  match e with 
+  | VAR v     => VAR (STyVar s v) 
+  | APP e1 e2 => APP (STyExp s e1) (STyExp s e2) 
+  | LAM e     => LAM (STyExp s e) 
+  | TAPP e t' => cast (STyExp_cast1 _ _ _ _) (TAPP (STyExp s e) (STyT s t')) 
+  | TLAM e    => TLAM (cast (STyExp_cast2 _ _ _) (STyExp (STyL s) e))
+  end.
+
+Definition Sub Γ Γ' := ∀ τ, Var Γ τ → Exp Γ' τ.
+
+Definition idSub {Γ} : Sub Γ Γ := @VAR Γ.
+
+(*
+Program Definition consSub {Γ Γ' τ} (e : Exp Γ' τ)
+        (s : Sub Γ Γ') : Sub (τ :: Γ) Γ' :=
+  λ _ v, match v with
+         | ZV    => e
+         | SV v' => s _ v'
+         end.
+*)
+
+Equations consSub {Γ Γ' τ} (e : Exp Γ' τ) (s : Sub Γ Γ')
+          τ' (v : Var (τ :: Γ) τ') : Exp Γ' τ' :=
+  consSub e s τ' ZV      := e;
+  consSub e s τ' (SV v') := s _ v'.
+
+Notation "{| e ; .. ; f |}" := (consSub e .. (consSub f idSub) ..).
+
+Definition tlSub {Γ Γ' τ} (s : Sub (τ :: Γ) Γ') : Sub Γ Γ' :=
+  λ τ' v => s τ' (SV v).
+Definition hdSub {Γ Γ' τ} (s : Sub (τ :: Γ) Γ') : Exp Γ' τ := s τ ZV.
+
+Definition Ren Γ Γ' := ∀ τ, Var Γ τ → Var Γ' τ.
+
+Definition idRen {Γ} : Ren Γ Γ := λ _, id.
+
+Definition tlRen {Γ Γ' τ} (r : Ren (τ :: Γ) Γ') : Ren Γ Γ' :=
+  λ τ' v => r τ' (SV v).
+Definition hdRen {Γ Γ' τ} (r : Ren (τ :: Γ) Γ') : Var Γ' τ := r τ ZV.
+
+Definition skip1 {Γ τ} : Ren Γ (τ :: Γ) := λ _, SV.
+
+Equations skipn {Γ} Γ' : Ren Γ (Γ' ++ Γ) :=
+  skipn []        := λ _, id;
+  skipn (x :: xs) := λ τ v, SV (skipn xs τ v).
+
+(*
+Program Definition RTmL {Γ Γ' τ} (r : Ren Γ Γ') :
+        Ren (τ :: Γ) (τ :: Γ') :=
+  λ _ v, match v with
+         | ZV    => ZV
+         | SV v' => SV (r _ v')
+         end.
+*)
+
+(* This version gives better rewriting equations. *)
+Equations RTmL {Γ Γ' τ} (r : Ren Γ Γ')
+          τ' (v : Var (τ :: Γ) τ') : Var (τ :: Γ') τ' :=
+  RTmL r τ' ZV      := ZV;
+  RTmL r τ' (SV v') := SV (r _ v').
+
+Lemma RTmL_id {Γ τ} : @RTmL Γ Γ τ (λ _, id) = λ _, id.
+Proof.
+  extensionality τ'.
+  extensionality v.
+  dependent induction v.
+  - now rewrite RTmL_equation_1.
+  - now rewrite RTmL_equation_2.
+Qed.
+
+Fixpoint RTmExp {Γ Γ' τ} (r : Ren Γ Γ') (e : Exp Γ τ) : Exp Γ' τ :=
+  match e with
+  | VAR v     => VAR (r _ v)
+  | APP e1 e2 => APP (RTmExp r e1) (RTmExp r e2)
+  | LAM e     => LAM (RTmExp (RTmL r) e)
+  end.
+
+Definition wk {Γ τ τ'} : Exp Γ τ → Exp (τ' :: Γ) τ := RTmExp (λ _, SV).
+
+(*
+Program Definition STmL {Γ Γ' τ} (s : Sub Γ Γ') :
+        Sub (τ :: Γ) (τ :: Γ') :=
+  λ _ v, match v with
+         | ZV    => VAR ZV
+         | SV v' => wk (s _ v')
+         end.
+*)
+
+Equations STmL {Γ Γ' τ} (s : Sub Γ Γ') τ' (v : Var (τ :: Γ) τ') :
+  Exp (τ :: Γ') τ' :=
+  STmL _ τ' ZV      := VAR ZV;
+  STmL _ τ' (SV v') := wk (s _ v').
+
+Fixpoint STmExp {Γ Γ' τ} (s : Sub Γ Γ') (e : Exp Γ τ) : Exp Γ' τ :=
+  match e with
+  | VAR v     => s _ v
+  | APP e1 e2 => APP (STmExp s e1) (STmExp s e2)
+  | LAM e     => LAM (STmExp (STmL s) e)
+  end.
+
+Inductive Ev : ∀ {τ}, Exp [] τ → Exp [] τ → Prop :=
+  | EvAbs t1 t2 (e : Exp [t1] t2) : Ev (LAM e) (LAM e)
+  | EvApp t1 t2 e v w (e1 : Exp [] (t1 ⟶ t2)) e2 :
+    Ev e1 (LAM e) → Ev e2 w → Ev (STmExp {| w |} e) v →
+    Ev (APP e1 e2) v.
+
+(* Notation "Γ ⊢ e ： τ" := (Judgment Γ τ e) (at level 80, no associativity). *)
+
+Definition identity Γ τ : Exp Γ (τ ⟶ τ) := LAM (VAR ZV).
+
+Definition compose {Γ τ τ' τ''}
+           (f : Exp Γ (τ' ⟶ τ''))
+           (g : Exp Γ (τ ⟶ τ')) : Exp Γ (τ ⟶ τ'') :=
+  LAM (APP (wk f) (APP (wk g) (VAR ZV))).
+
+Definition RcR {Γ Γ' Γ''} (r : Ren Γ' Γ'') (r' : Ren Γ Γ') :=
+  (λ τ v, r τ (r' τ v)) : Ren Γ Γ''.
+
+Definition ScR {Γ Γ' Γ''} (s : Sub Γ' Γ'') (r : Ren Γ Γ') :=
+  (λ τ v, s τ (r τ v)) : Sub Γ Γ''.
+
+Definition RcS {Γ Γ' Γ''} (r : Ren Γ' Γ'') (s : Sub Γ Γ') :=
+  (λ τ v, RTmExp r (s τ v)) : Sub Γ Γ''.
+
+Definition ScS {Γ Γ' Γ''} (s : Sub Γ' Γ'') (s' : Sub Γ Γ') :=
+  (λ τ v, STmExp s (s' τ v)) : Sub Γ Γ''.
+
+Lemma LiftRcR Γ Γ' Γ'' τ (r : Ren Γ' Γ'') (r' : Ren Γ Γ') :
+  RTmL (τ := τ) (RcR r r') = RcR (RTmL r) (RTmL r').
+Proof.
+  extensionality τ'.
+  extensionality v.
+  now dependent induction v.
+Qed.
+
+Corollary tlRen_skip1 Γ τ τ' :
+  @tlRen _ (τ :: τ' :: Γ) _ skip1 = RcR skip1 skip1.
+Proof. reflexivity. Qed.
